src/ocaml-output/FStar_TypeChecker_NBETerm.ml
@@ -1622,83 +1622,64 @@ let lift_binary :
 let unary_op :
   'a .
     (arg -> 'a FStar_Pervasives_Native.option) ->
-      ('a -> t) -> args -> t FStar_Pervasives_Native.option
+      ('a -> t) ->
+        FStar_Syntax_Syntax.universes ->
+          args -> t FStar_Pervasives_Native.option
   =
   fun as_a ->
     fun f ->
-      fun args1 ->
-        let uu___ = FStar_Compiler_List.map as_a args1 in lift_unary f uu___
+      fun us ->
+        fun args1 ->
+          let uu___ = FStar_Compiler_List.map as_a args1 in
+          lift_unary f uu___
 let binary_op :
   'a .
     (arg -> 'a FStar_Pervasives_Native.option) ->
-      ('a -> 'a -> t) -> args -> t FStar_Pervasives_Native.option
+      ('a -> 'a -> t) ->
+        FStar_Syntax_Syntax.universes ->
+          args -> t FStar_Pervasives_Native.option
   =
   fun as_a ->
     fun f ->
-      fun args1 ->
-        let uu___ = FStar_Compiler_List.map as_a args1 in lift_binary f uu___
+      fun _us ->
+        fun args1 ->
+          let uu___ = FStar_Compiler_List.map as_a args1 in
+          lift_binary f uu___
 let (unary_int_op :
   (FStar_BigInt.t -> FStar_BigInt.t) ->
-    args -> t FStar_Pervasives_Native.option)
+    FStar_Syntax_Syntax.universes -> args -> t FStar_Pervasives_Native.option)
   =
   fun f ->
     unary_op arg_as_int
       (fun x -> let uu___ = f x in embed e_int bogus_cbs uu___)
 let (binary_int_op :
   (FStar_BigInt.t -> FStar_BigInt.t -> FStar_BigInt.t) ->
-    args -> t FStar_Pervasives_Native.option)
+    FStar_Syntax_Syntax.universes -> args -> t FStar_Pervasives_Native.option)
   =
   fun f ->
     binary_op arg_as_int
       (fun x -> fun y -> let uu___ = f x y in embed e_int bogus_cbs uu___)
 let (unary_bool_op :
-  (Prims.bool -> Prims.bool) -> args -> t FStar_Pervasives_Native.option) =
+  (Prims.bool -> Prims.bool) ->
+    FStar_Syntax_Syntax.universes -> args -> t FStar_Pervasives_Native.option)
+  =
   fun f ->
     unary_op arg_as_bool
       (fun x -> let uu___ = f x in embed e_bool bogus_cbs uu___)
 let (binary_bool_op :
   (Prims.bool -> Prims.bool -> Prims.bool) ->
-    args -> t FStar_Pervasives_Native.option)
+    FStar_Syntax_Syntax.universes -> args -> t FStar_Pervasives_Native.option)
   =
   fun f ->
     binary_op arg_as_bool
       (fun x -> fun y -> let uu___ = f x y in embed e_bool bogus_cbs uu___)
 let (binary_string_op :
   (Prims.string -> Prims.string -> Prims.string) ->
-    args -> t FStar_Pervasives_Native.option)
+    FStar_Syntax_Syntax.universes -> args -> t FStar_Pervasives_Native.option)
   =
   fun f ->
     binary_op arg_as_string
       (fun x -> fun y -> let uu___ = f x y in embed e_string bogus_cbs uu___)
-let mixed_binary_op_no_univs :
-  'a 'b 'c .
-    (arg -> 'a FStar_Pervasives_Native.option) ->
-      (arg -> 'b FStar_Pervasives_Native.option) ->
-        ('c -> t) ->
-          ('a -> 'b -> 'c FStar_Pervasives_Native.option) ->
-            args -> t FStar_Pervasives_Native.option
-  =
-  fun as_a ->
-    fun as_b ->
-      fun embed_c ->
-        fun f ->
-          fun args1 ->
-            match args1 with
-            | a1::b1::[] ->
-                let uu___ =
-                  let uu___1 = as_a a1 in
-                  let uu___2 = as_b b1 in (uu___1, uu___2) in
-                (match uu___ with
-                 | (FStar_Pervasives_Native.Some a2,
-                    FStar_Pervasives_Native.Some b2) ->
-                     let uu___1 = f a2 b2 in
-                     (match uu___1 with
-                      | FStar_Pervasives_Native.Some c1 ->
-                          let uu___2 = embed_c c1 in
-                          FStar_Pervasives_Native.Some uu___2
-                      | uu___2 -> FStar_Pervasives_Native.None)
-                 | uu___1 -> FStar_Pervasives_Native.None)
-            | uu___ -> FStar_Pervasives_Native.None
 let mixed_binary_op :
   'a 'b 'c .
     (arg -> 'a FStar_Pervasives_Native.option) ->
